Replace Valuation with ProgramState.

CrIdentifiers.v
@@ -19,19 +19,19 @@ Definition HeaderMap := Header -> uint8.
 Definition StateVarMap := StateVar -> uint8.
 Definition CtrlPlaneConfigNameMap := CtrlPlaneConfigName -> uint8.
 
-Definition hdr_update (s: Header -> uint8) (x: Header) (v: uint8) : (Header -> uint8) :=
+Definition update_hdr_map (s: Header -> uint8) (x: Header) (v: uint8) : (Header -> uint8) :=
   fun y => match x, y with
             | HeaderCtr x_name, HeaderCtr y_name => if string_dec x_name y_name then v else s y
            end.
 
-Definition state_update (s: StateVar -> uint8) (x: StateVar) (v: uint8) : (StateVar -> uint8) :=
+Definition update_state_map (s: StateVar -> uint8) (x: StateVar) (v: uint8) : (StateVar -> uint8) :=
   fun y => match x, y with
             | StateVarCtr x_name, StateVarCtr y_name => if string_dec x_name y_name then v else s y
            end.
 
-(* The valuation is a record containing three maps:,
+(* The ProgramState is a record containing three maps:,
    one each for mapping headers/statevars/ctrlplaneconfigs to their current values *)
-Record Valuation := {
+Record ProgramState := {
   ctrl_plane_map : CtrlPlaneConfigNameMap;
   header_map : HeaderMap;
   state_var_map : StateVarMap
