CrSemantics.v
@@ -8,7 +8,7 @@ From MyProject Require Export CrIdentifiers.
 (* TODO: fill out eval_transformer body at the end,
    right now, we are just specifying it as a function that
    goes from previous valuation to new one *)
-Parameter eval_transformer : Transformer -> Valuation -> Valuation.
+Parameter eval_transformer : Transformer -> ProgramState -> ProgramState.
 
 (* A Transformer is a list of match-action rules,
    where each rule is either sequential or parallel,
@@ -17,18 +17,18 @@ Parameter eval_transformer : Transformer -> Valuation -> Valuation.
 (* Function to evaluate a match-action rule,
    meaning header ops within an action are evaluated
    according to the type of the rule (sequential or parallel) *)
-Parameter eval_match_action_rule : MatchActionRule -> Valuation -> Valuation.
+Parameter eval_match_action_rule : MatchActionRule -> ProgramState -> ProgramState.
 
 (* Function to evaluate a sequential match-action rule,
    meaning header ops within an action are evaluated sequentially *)
-Parameter eval_seq_rule : MatchActionRule -> Valuation -> Valuation.
+Parameter eval_seq_rule : MatchActionRule -> ProgramState -> ProgramState.
 
 (* Function to evaluate a parallel match-action rule,
    meaning header ops within an action are evaluated in parallel *)
-Parameter eval_par_rule : MatchActionRule -> Valuation -> Valuation.
+Parameter eval_par_rule : MatchActionRule -> ProgramState -> ProgramState.
 
 (* Expression version of a header operation, meaning side-effect-free and stateless *)
-Definition eval_hdr_op_expr (op : HdrOp) (v : Valuation) : uint8 :=
+Definition eval_hdr_op_expr (op : HdrOp) (v : ProgramState) : uint8 :=
     match op with
     | StatefulOp f arg1 arg2 target => apply_bin_op f (function_argument_to_uint8 arg1 v) (function_argument_to_uint8 arg2 v)
     | StatelessOp f arg1 arg2 target => apply_bin_op f (function_argument_to_uint8 arg1 v) (function_argument_to_uint8 arg2 v)
@@ -36,21 +36,20 @@ Definition eval_hdr_op_expr (op : HdrOp) (v : Valuation) : uint8 :=
 
 (* Function to evaluate a header operation,
    meaning we apply the operation to a previous valuation to get a new one *)
-Definition eval_hdr_op (op : HdrOp) (input_valuation : Valuation) : Valuation :=
+Definition eval_hdr_op (op : HdrOp) (input_valuation : ProgramState) : ProgramState :=
     match op with
     | StatefulOp f arg1 arg2 target =>
         let new_state :=
            let op_output := eval_hdr_op_expr op input_valuation in
-            state_update (state_var_map input_valuation) target op_output in
+            update_state_map (state_var_map input_valuation) target op_output in
             {| ctrl_plane_map := ctrl_plane_map input_valuation;   (* Leave this unchanged *)
                header_map := header_map input_valuation;           (* Leave this unchanged *)
                state_var_map := new_state |}                       (* Modify this *)
     | StatelessOp f arg1 arg2 target =>
         let new_hdr :=
            let op_output := eval_hdr_op_expr op input_valuation in
-            hdr_update (header_map input_valuation) target op_output in
+            update_hdr_map (header_map input_valuation) target op_output in
             {| ctrl_plane_map := ctrl_plane_map input_valuation;   (* Leave this unchanged *)
                header_map := new_hdr;                              (* Modify this *)
                state_var_map := state_var_map input_valuation |}   (* Leave this unchanged *)
     end.
-(*TODO: Maybe figure out a way to unify parsing and header manipulation into seq and par transformers respectively. *)
