CrTransformer.v
@@ -19,7 +19,7 @@ Inductive FunctionArgument :=
   | StatefulArg (s : StateVar).
 
 (* lookup a function's argument *)
-Definition function_argument_to_uint8 (arg : FunctionArgument) (valuation : Valuation) : uint8 :=
+Definition function_argument_to_uint8 (arg : FunctionArgument) (valuation : ProgramState) : uint8 :=
   match arg with
   | CtrlPlaneArg c => valuation.(ctrl_plane_map) c
   | HeaderArg h    => valuation.(header_map) h
@@ -46,15 +46,3 @@ Inductive MatchActionRule :=
   | Par (h : Header) (start_index : uint8) (end_index : uint8) (pat : list bool) (action : list HdrOp).
 
 Definition Transformer : Type := list MatchActionRule.
-
-(* Example header *)
-Definition example_header1 : Header := HeaderCtr "hdr1"%string.
-
-(* An example transformer *)
-Definition example_transformer : Transformer :=
-  [
-    Seq example_header1 zero (repr 10%Z) [true; false; true] 
-      [StatefulOp  AddOp (HeaderArg example_header1) (ConstantArg (repr 5%Z)) (StateVarCtr "state1"%string)];
-    Par example_header1 zero (repr 10%Z) [false; true; false] 
-      [StatelessOp AddOp (HeaderArg example_header1) (ConstantArg (repr 3%Z)) (HeaderCtr "hdr2"%string)]
-  ].
